Added all the variants for #281, they all work well now

examples/bug-reports/bug281.fst
@@ -46,6 +46,12 @@ val lemma : s:sub -> e:exp -> Lemma (esubst (sub_elam s) (eesh e)
                                    = eesh (esubst s e))
 let lemma s e = admit()
 
+(* Version without type : succeeds after a random time or fails *)
+let plouf0 s f =lemma (sub_elam (sub_elam s)) (eesh (eesh f));
+                lemma (sub_elam s) (eesh f);
+                lemma (s) (f);
+                assert(esubst (sub_elam (sub_elam (sub_elam s))) (test f) = test (esubst s f))
+
 (* Succeeds after ~2-6sec *)
 val plouf1 : s:sub -> f:exp -> Tot unit
 let plouf1 s f =lemma (sub_elam (sub_elam s)) (eesh (eesh f));
@@ -58,5 +64,11 @@ let plouf1 s f =lemma (sub_elam (sub_elam s)) (eesh (eesh f));
 val plouf2 : s:sub -> f :exp ->
   Lemma (esubst (sub_elam (sub_elam (sub_elam s))) (test f) = test (esubst s f))
 let plouf2 s f =lemma (sub_elam (sub_elam s)) (eesh (eesh f));
+                lemma (sub_elam s) (eesh f);
+                lemma (s) (f)
+
+(* another try, with raw encoding of the wp *)
+val plouf4 : s:sub -> f:exp -> PURE unit (fun (p:pure_post unit) -> (esubst (sub_elam (sub_elam (sub_elam s))) (test f) = test (esubst s f)) ==> p ())
+let plouf4 s f =lemma (sub_elam (sub_elam s)) (eesh (eesh f));
                 lemma (sub_elam s) (eesh f);
                 lemma (s) (f)
